cfrontend/Ctypingsec.v
@@ -1,0 +1,361 @@
+
+Require Import String.
+Require Import Coqlib Maps Integers Floats Errors.
+Require Import AST Linking.
+Require Import Values Memory Globalenvs Events.
+Require Import Ctypes Ctyping Cop Csyntax Csem.
+
+Local Open Scope error_monad_scope.
+
+(**
+    Security typechecker
+    Assumes that normal typechecking has already passed, and thus that types already match, ignoring security annotations.
+    Typechecks security annotations (trusting only that variable/function declarations have the correct security type).
+    Performs implicit classification.
+    Introduces security builtin operations.
+    Replaces security types for void pointers.
+**)
+
+(** Utils **)
+
+Fixpoint type_has_secret (ty: type) : bool :=
+  match ty with
+  | Tvoid => false
+  | Tint _ _ a => a.(attr_secret)
+  | Tlong _ a => a.(attr_secret)
+  | Tfloat _ a => a.(attr_secret)
+  | Tpointer t a => a.(attr_secret) || type_has_secret t
+  | Tarray t _ a => a.(attr_secret) || type_has_secret t
+  | Tfunction _ _ _ => false
+  | Tstruct _ a => a.(attr_secret)
+  | Tunion _ a => a.(attr_secret)
+  end.
+
+Definition make_public_attr (a : attr) : attr :=
+  {| attr_volatile := a.(attr_volatile);
+     attr_secret := false;
+     attr_alignas := a.(attr_alignas);
+  |}.
+  
+Definition set_attr_secret (sec:bool) (a : attr) : attr :=
+  {| attr_volatile := a.(attr_volatile);
+     attr_secret := sec;
+     attr_alignas := a.(attr_alignas);
+  |}.
+  
+Definition type_is_public (ty: type) : bool :=
+  negb (type_is_secret ty).
+  
+Definition make_public_type (ty: type) : type :=
+  change_attributes make_public_attr ty.
+
+Definition check_public (t: type) : res unit :=
+  if type_is_public t then OK tt else Error (msg "unsupported secure control flow").
+  
+Definition check_secret (t: type) : res unit :=
+  if type_is_secret t then OK tt else Error (msg "expected secret type").
+
+(** builtins **)
+
+Definition external_new_int8_array : external_function :=
+    EF_builtin "new_int8_array" (mksignature (cons AST.Tlong nil) (Some Tptr) cc_default).
+Definition builtin_new_int8_array (sz: expr) (rty : type) : expr :=
+    Ebuiltin external_new_int8_array (Tcons (typeof sz) Tnil) (Econs sz Enil) rty.
+
+Definition external_add_int8 : external_function :=
+    EF_builtin "add_int8" (mksignature (cons Tptr (cons Tptr nil)) (Some Tptr) cc_default).
+Definition builtin_add_int8 (e1 e2: expr) : expr :=
+    Ebuiltin external_add_int8 (Tcons (typeof e1) (Tcons (typeof e2) Tnil)) (Econs e1 (Econs e2 Enil)) (typeof e1).
+
+(** Security typechecker **)
+
+(*TODO undefined*)
+Definition secure_classify (t: type) (e: expr) : res expr := OK e.
+
+(*TODO undefined*)
+Definition secure_convert (rt t: type) (e: expr) : res expr := OK e.
+
+Definition is_public_cast (rt: type) (t: type) (e: expr) : bool :=
+    negb (type_has_secret rt) && negb (type_has_secret t).
+
+Definition public_cast (rt: type) (t: type) (e: expr) : res expr :=
+   if is_public_cast rt t e then OK e else Error (msg "unsupported non-public cast").
+
+(* Disallow any cast involving security types besides direct classifies or conversions *)
+(* TODO: casts are still not safe! e.g. int => void => int secret, int secret* => int** *)
+Definition secure_cast (rt: type) (t: type) (e:expr) : res expr :=
+    match (type_is_secret rt,type_is_secret t) with
+    | (false,false) => OK e
+    | (true,false) => do e' <- public_cast (make_public_type rt) t e; secure_classify t e'
+    | (false,true) => Error (msg "unsupported cast from secure to non-secure type, try declassify")
+    | (true,true) => secure_convert rt t e
+    end.
+
+Definition secure_binarith_type (ty1 ty2: type) (m: string): res type :=
+  match classify_binarith ty1 ty2 with
+  | bin_case_i sg => OK (Tint I32 sg (snoattr (type_is_secret ty1 || type_is_secret ty2)))
+  | bin_case_l sg => OK (Tlong sg (snoattr (type_is_secret ty1 || type_is_secret ty2)))
+  | bin_case_f => OK (Tfloat F64 (snoattr (type_is_secret ty1 || type_is_secret ty2)))
+  | bin_case_s => OK (Tfloat F32 (snoattr (type_is_secret ty1 || type_is_secret ty2)))
+  | bin_default   => Error (msg m)
+  end.
+
+Definition secure_binarith_int_type (ty1 ty2: type) (m: string): res type :=
+  match classify_binarith ty1 ty2 with
+  | bin_case_i sg => OK (Tint I32 sg (snoattr (type_is_secret ty1 || type_is_secret ty2)))
+  | bin_case_l sg => OK (Tlong sg (snoattr (type_is_secret ty1 || type_is_secret ty2)))
+  | _ => Error (msg m)
+  end.
+
+Definition secure_shift_op_type (ty1 ty2: type) (m: string): res type :=
+  match classify_shift ty1 ty2 with
+  | shift_case_ii sg | shift_case_il sg => OK (Tint I32 sg (snoattr (type_is_secret ty1 || type_is_secret ty2)))
+  | shift_case_li sg | shift_case_ll sg => OK (Tlong sg (snoattr (type_is_secret ty1 || type_is_secret ty2)))
+  | shift_default => Error (msg m)
+  end.
+
+Definition secure_comparison_type (ty1 ty2: type) (m: string): res type :=
+  match classify_binarith ty1 ty2 with
+  | bin_default => Error (msg m)
+  | c => OK (Tint I32 Signed (snoattr (type_is_secret ty1 || type_is_secret ty2)))
+  end.
+
+Definition secure_type_binop (op: binary_operation) (ty1 ty2: type) : res type :=
+  match op with
+  | Oadd => secure_binarith_type ty1 ty2 "operator +"
+  | Osub => secure_binarith_type ty1 ty2 "operator infix -"
+  | Omul => secure_binarith_type ty1 ty2 "operator infix *"
+  | Odiv => secure_binarith_type ty1 ty2 "operator /"
+  | Omod => secure_binarith_int_type ty1 ty2 "operator %"
+  | Oand => secure_binarith_int_type ty1 ty2 "operator &"
+  | Oor  => secure_binarith_int_type ty1 ty2 "operator |"
+  | Oxor => secure_binarith_int_type ty1 ty2 "operator ^"
+  | Oshl => secure_shift_op_type ty1 ty2 "operator <<"
+  | Oshr => secure_shift_op_type ty1 ty2 "operator >>"
+  | Oeq  => secure_comparison_type ty1 ty2 "operator =="
+  | One  => secure_comparison_type ty1 ty2 "operator !="
+  | Olt  => secure_comparison_type ty1 ty2 "operator <"
+  | Ogt  => secure_comparison_type ty1 ty2 "operator >"
+  | Ole  => secure_comparison_type ty1 ty2 "operator <="
+  | Oge  => secure_comparison_type ty1 ty2 "operator >="
+  end.
+
+(*TODO undefined *)
+Definition retype_secure_type (t: type) : res type := OK t.
+
+Fixpoint retype_secure_typelist (ts: typelist) : res typelist :=
+    match ts with
+    | Tnil => OK Tnil
+    | Tcons x xs => do x' <- retype_secure_type x; do xs' <- retype_secure_typelist xs; OK (Tcons x' xs')
+    end.
+
+(*TODO undefined*)
+Definition secure_binop_expr (op: binary_operation) (t: type) (e1 e2 : expr) : res expr :=
+  do _ <- check_secret t;
+  match t with
+  | Tint I8 Signed _ => OK (builtin_add_int8 e1 e2)
+  | _ => Error (msg "unsupported secure binop")
+  end.
+
+Definition secure_binop (op : binary_operation) (t1 t2 t: type) (e1 e2: expr): res (expr * type) :=
+  match (type_is_secret t1,type_is_secret t2) with
+  | (false,false) => (* assumes that casts preserve non-top-level security tags*)
+      do t' <- retype_secure_type t;
+      OK (Ebinop op e1 e2 t',t)
+  | _ =>
+      do t' <- secure_type_binop op t1 t2;
+      do e1' <- secure_cast t' t1 e1;
+      do e2' <- secure_cast t' t2 e2;
+      do e' <- secure_binop_expr op t' e1' e2';
+      OK (e',t')
+  end.
+    
+
+(*TODO undefined *)
+(* returns a typechecked expression with security annotations already removed, and the typechecked security type *)
+Fixpoint retype_secure_expr (ce: composite_env) (e: typenv) (a: expr) : res (expr * type) :=
+  match a with
+  | Eval v t => OK (a,t)
+  | Evar x t => OK (a,t)
+  | Efield r f t =>
+      do (r',tr') <- retype_secure_expr ce e r;
+      do t' <- type_field ce tr' f;
+      do t'' <- retype_secure_type t';
+      OK (Efield r f t'',t')
+  | Evalof r t =>
+      do (r',tr') <- retype_secure_expr ce e r;
+      OK (Evalof r' (typeof r'),tr')
+  (*| Ederef r t => if type_is_public (typeof r)
+      then
+          do r' <- retype_secure_expr r;
+          do t' <- type_deref (typeof r);
+          do t'' <- retype_secure_type t';
+          OK (Ederef r' t'')
+      else
+          do (x,eoff) <- match r with
+          | Evar x xt => 
+          | Ebinop Oadd (Evar x xt) e2 _ =>
+          | _ => Error (msg "unsupported array projection")
+          end;*)
+  | Eaddrof l t =>
+      do (l',lt') <- retype_secure_expr ce e l;
+      OK (Eaddrof l' (Tpointer (typeof l) noattr),Tpointer lt' noattr)
+(*  | Eunop op r1 t =>
+      do (r1',tr1') <- retype_secure_expr ce e r1;*)    
+  | Ebinop op r1 r2 t =>
+      do (r1',tr1') <- retype_secure_expr ce e r1;
+      do (r2',tr2') <- retype_secure_expr ce e r2;
+      secure_binop op tr1' tr2' t r1' r2'
+  | _ => Error (msg "undefined")
+  end.
+
+Definition retype_secure_public_expr (ce: composite_env) (e: typenv) (a: expr) : res expr :=
+    do _ <- check_public (typeof a);
+    do (e',_) <- retype_secure_expr ce e a;
+    OK e'.
+
+Fixpoint retype_secure_stmt (ce: composite_env) (e: typenv) (rt: type) (s: statement) : res statement :=
+  match s with
+  | Sskip => OK Sskip
+  | Sdo a => do (a',_) <- retype_secure_expr ce e a; OK (Sdo a')
+  | Ssequence s1 s2 =>
+      do s1' <- retype_secure_stmt ce e rt s1;
+      do s2' <- retype_secure_stmt ce e rt s2;
+      OK (Ssequence s1' s2')
+  | Sifthenelse a s1 s2 =>
+      do a' <- retype_secure_public_expr ce e a;
+      do s1' <- retype_secure_stmt ce e rt s1; do s2' <- retype_secure_stmt ce e rt s2;
+      OK (Sifthenelse a' s1' s2')
+  | Swhile a s =>
+      do a' <- retype_secure_public_expr ce e a;
+      do s' <- retype_secure_stmt ce e rt s;
+      OK (Swhile a' s')
+  | Sdowhile a s =>
+      do a' <- retype_secure_public_expr ce e a;
+      do s' <- retype_secure_stmt ce e rt s;
+      do _ <- check_public (typeof a);
+      OK (Sdowhile a' s')
+  | Sfor s1 a s2 s3 =>
+      do a' <- retype_secure_public_expr ce e a;
+      do s1' <- retype_secure_stmt ce e rt s1;
+      do s2' <- retype_secure_stmt ce e rt s2;
+      do s3' <- retype_secure_stmt ce e rt s3;
+      OK (Sfor s1' a' s2' s3')
+  | Sbreak => OK Sbreak
+  | Scontinue => OK Scontinue
+  | Sreturn None => OK (Sreturn None)
+  | Sreturn (Some a) =>
+      do (a',t') <- retype_secure_expr ce e a;
+      do a'' <- secure_cast rt t' a';
+      OK (Sreturn (Some a''))
+  | Sswitch a sl =>
+      do a' <- retype_secure_public_expr ce e a;
+      do sl' <- retype_secure_lblstmts ce e rt sl;
+      OK (Sswitch a' sl')
+  | Slabel lbl s => do s' <- retype_secure_stmt ce e rt s; OK (Slabel lbl s')
+  | Sgoto lbl => OK (Sgoto lbl)
+  end
+with retype_secure_lblstmts (ce: composite_env) (e: typenv) (rt: type) (sl: labeled_statements) : res labeled_statements :=
+  match sl with
+  | LSnil => OK LSnil
+  | LScons case s sl =>
+      do s' <- retype_secure_stmt ce e rt s; do sl' <- retype_secure_lblstmts ce e rt sl;
+      OK (LScons case s' sl')
+  end.
+
+(*TODO undefined *)
+Definition retype_secure_fn_params (ps : list (ident * type)) : res (list (ident * type)) := OK ps.
+
+(*TODO fill with more types *)
+Definition initialize_secure_var (n: ident) (t t': type) : res statement :=
+    match t with
+    | Tint I8 Signed a => OK Sskip
+    | Tarray bt sz a => if a.(attr_secret)
+        then if type_has_secret bt then Error (msg "unsupported secret array") else
+        do blt <- match bt with
+        | Tint I8 Signed _ => OK (builtin_new_int8_array (Eval (Vlong (Int64.repr sz)) (Tlong Signed noattr)) t')
+        | _ => Error (msg "unsupported secret array")
+        end;
+        OK (Sdo (Eassign (Evar n t') blt t'))
+        else OK Sskip
+    | _ => Error (msg "unsupported secure variable type")
+    end.
+
+Definition retype_secure_fn_var (n : ident) (t: type) : res ((ident * type) * statement) :=
+    do t' <- retype_secure_type t;
+    do s' <- initialize_secure_var n t t';
+    OK (pair (pair n t') s').
+
+(*TODO undefined *)
+Definition retype_secure_fn_vars (ps : list (ident * type)) : res (list (ident * type) * statement) := OK (ps,Sskip).
+
+Definition retype_secure_function (ce: composite_env) (e: typenv) (f: function) : res function :=
+  let e := bind_vars (bind_vars e f.(fn_params)) f.(fn_vars) in
+  do s' <- retype_secure_stmt ce e f.(fn_return) f.(fn_body);
+  do ret' <- retype_secure_type f.(fn_return);
+  do params' <- retype_secure_fn_params f.(fn_params);
+  do (vars',s0) <- retype_secure_fn_vars f.(fn_vars);
+  OK (mkfunction ret' f.(fn_callconv) params' vars' (Ssequence s0 s')).         
+
+Definition retype_secure_fundef (ce: composite_env) (e: typenv) (fd: fundef) : res fundef :=
+  match fd with
+  | Internal f => do f' <- retype_secure_function ce e f; OK (Internal f')
+  | External id args res cc =>
+      do args' <- retype_secure_typelist args;
+      do res' <- retype_secure_type res;
+      OK (External id args' res' cc)
+  end.
+
+(* TODO: reject global secure variables *)
+Definition typecheck_secure_program (p: program) : res program :=
+  let e := bind_globdef (PTree.empty _) p.(prog_defs) in
+  let ce := p.(prog_comp_env) in
+  do tp <- transform_partial_program (retype_secure_fundef ce e) p;
+  OK {| prog_defs := tp.(AST.prog_defs);
+        prog_public := p.(prog_public);
+        prog_main := p.(prog_main);
+        prog_types := p.(prog_types);
+        prog_comp_env := ce;
+        prog_comp_env_eq := p.(prog_comp_env_eq) |}.
+
+(** Remove security qualifiers **)
+
+(*Definition remsec_type (t : type) : res type := OK t.
+
+Definition remsec_fundef (n: ident) (f: fundef) : res fundef := OK f.
+    
+Definition remsec_globdef (n: ident) (t: type) : res type :=
+    remsec_type t.
+
+Definition remsec_member (xy : ident * type) : res (ident * type) := 
+    match xy with
+    | pair x y => do y' <- remsec_type y; OK (pair x y')
+    end.
+
+Fixpoint remsec_members (xs : list (ident * type)) : res (list (ident * type)) := 
+    match xs with
+    | nil => OK nil
+    | x :: xs => do x' <- remsec_member x; do xs' <- remsec_members xs; OK (x'::xs')
+    end.
+
+Definition remsec_composite_definition (c: composite_definition) : res composite_definition :=
+    match c with
+    | Composite id su ms a =>
+        do ms' <- (remsec_members ms);
+        OK (Composite id su ms' (make_public_attr a))
+    end.
+
+Fixpoint remsec_composite_definitions (xs : list composite_definition) : res (list composite_definition) := 
+    match xs with
+    | nil => OK nil
+    | x :: xs => do x' <- remsec_composite_definition x; do xs' <- remsec_composite_definitions xs; OK (x'::xs')
+    end.
+
+Definition remsec_program (p: program) : res program :=
+    do tp <- transform_partial_program2 remsec_fundef remsec_globdef p;
+    OK {| prog_defs := tp.(AST.prog_defs);
+          prog_public := p.(prog_public);
+          prog_main := p.(prog_main);
+          prog_types := p.(prog_types);
+          prog_comp_env := p.(prog_comp_env);
+          prog_comp_env_eq := p.(prog_comp_env_eq) |}.*)
